Weidenbach_Book/IsaSAT/IsaSAT_Garbage_Collect_LLVM.thy
@@ -178,18 +178,18 @@ sepref_def rewatch_heur_st_code
 
 sepref_register isasat_GC_clauses_wl_D
 (*
-lemma schedule_next_inprocessing_st_alt_def:
-  \<open>schedule_next_inprocessing_st b S =
+lemma schedule_next_pure_lits_st_alt_def:
+  \<open>schedule_next_pure_lits_st b S =
       (let should_inprocess = should_inprocess_st S;
            (heur, S) = extract_heur_wl_heur S;
            (stats, S) = extract_stats_wl_heur S;
            (lcount, S) = extract_lcount_wl_heur S;
            bc = current_restart_phase heur;
-           heur = if b \<and> should_inprocess then (schedule_next_inprocessing (heur)) else heur;
+           heur = if b \<and> should_inprocess then (schedule_next_pure_lits (heur)) else heur;
            _ = isasat_print_progress (if should_inprocess then 105 else 103) bc stats (lcount);
            S = update_heur_wl_heur heur (update_stats_wl_heur stats (update_lcount_wl_heur lcount S)) in
   S)\<close>
-  by (auto simp: schedule_next_inprocessing_st_def state_extractors split: isasat_int_splits
+  by (auto simp: schedule_next_pure_lits_st_def state_extractors split: isasat_int_splits
     intro!: ext)
 
 
